# Polynomials and Polynomial Rings
## 32)
We did this one in class

## 33)

Suppose $f(x)\in\mathbb{z}[x]$ is reducible over $\mathbb{Q}$. Thus
$f(x)=b(x)c(x)$, then by (29) we know we can multiply by the lcm of the
denominators of the coefficents to get a polynomial with integer coefficients,
and thus we have $kb(x)$ and $lc(x)$. Then $klf(x)=(kb(x))(lc(x))$...

## 34)
$2x^3+6x^2-15x-12$ We consider $p=3$ as $3|12$, $3|15$, $3|6$, and $3\nmid 2$,
and $9\nmid 12$, thus by thm 2.28 $f(x)$ is irreducible over $\mathbb{Q}$.

## 35)
**(a)**
since $p|f_0$ and $f_0=b_0c_0$, then $p|b_0c_0$ so $p|b_0$ or $p|c_0$.

**(b)**
$p\nmid c_v$ as $p\nmid f_n$ with $f_n=b_uc_v$, so $p\nmid b_uc_v$, and thus
$p\nmid b_u$ and $p\nmid c_v$.

**(c)**
$a_k=b_0c_k+b_1c_{k-1}+\ldots+b_kc_0$

**(d)**
Since we have shown that $p\nmid c_v$ and $p\nmid b_0$, then $p|b_0c_k$ is a
contradiction.

## 36)
**(a)**
Yes just multiply by $x-1$ to both sides, and things will cancel out.

**(b)**
$$
\phi_p(x+1)=\frac{(x+1)^p-1}{x}
$$
Then, $(x+1)^p$ follows binomial theorem, $(x+1)^p=\sum$

**(c)**
By ${p\choose x}=\frac{p!}{n!(p-n)!}$, $p\vert{p\choose n}$ so long as $n\neq
0$ and $n\neq p$. And, ${p \choose {p-1}}=p$, so $p^2\nmid {n \choose p-1}$.
Lastly, $p\nmid 1$, so $\Phi_p(x+1)$ satisfies Eisenstein's Irreducibility
Criterion and so is irreducible.

**(d)**
Assume for contradiction $\Phi_p(x)$ is reducible. Then, $\Phi_p(x)=g(x)h(x)$,
so $\Phi_p(x+1)=g(x+1)h(x+1)$, giving that $\Phi_p(x+1)$ is reducible, a
contradiction.

# Vector Spaces
## 3)
$E$ is the vector field ($V$), and $F$ is the scalar field ($F$).

Define the addition operation in the vector space by the addition operation of
$E$ as a field. Then, by $E$ a ring, $(E, +)$ forms an abelian group.

Define the scalar multiplication operation for the vector space by the
multiplication between elements of $E$. Then, properties (1) and (3) follows by
the distributive property of rings, property (2) follows from the
multiplication in a ring associativity, and property (4) follows by taking the
identity element of the  vector space to be the identity element of the field.

<!-- \documentclass{article} -->
<!-- \usepackage[utf8]{inputenc} -->
<!-- \usepackage[a4paper,bindingoffset=0.2in,% -->
            <!-- left=1in,right=1in,top=1in,bottom=1in,% -->
            <!-- footskip=.25in]{geometry} -->
<!-- \usepackage{amssymb} -->
<!-- \usepackage{amsmath} -->
<!-- \usepackage{graphicx} -->
<!-- \usepackage{subfig} -->
<!-- \usepackage{float} -->
<!-- \usepackage{enumitem} -->
<!-- \usepackage{pifont} -->

<!-- \newcommand{\cmark}{\ding{51}} -->
<!-- \newcommand{\xmark}{\ding{55}} -->
<!-- \captionsetup[subfigure]{labelformat=empty} -->

<!-- \title{Guass's Lemma, Eisenstein Criterion} -->
<!-- \author{Sean Richardson \tiny{and Minho Choi}} -->
<!-- \date{March 28, 2020} -->

<!-- \begin{document} -->

<!-- \maketitle -->

<!-- \section*{Problem 32} -->
<!-- \begin{enumerate}[label=(\alph*)] -->
    <!-- \item We need to find all the possible combinations of integers that sum up to $r+t$. So, we have: -->
    <!-- $$a_{r+t} = g_0 h_{r+t} + g_1 h_{r+t-1} + \dots + g_{r+t-1} h_1 + g_{r+t} h_0= \sum_{i=0}^{r+t} g_i h_{r+t-i}$$ -->

    <!-- \item Note that $g_r$ is the first coefficient of $G(x)$ that $p$ does not divide. This implies that every term in the summation from $g_0 h_{r+t}$ to $g_{r-1} h_{t+1}$ is divisible by $p$ because of $g_i$, where $0 \leq i \leq r-1$. Similarly, note that $h_t$ is the first coefficient of $H(x)$ that $p$ does not divide. This implies that every term in the summation from $g_{r+1} h_{t-1}$ to $g_{r+t} h_{0}$ is divisible by $p$ because of $h_j$, where $0 \leq j \leq t-1$. Hence, since $p \mid a_{r+t}$, $p$ divides the summation. Since $p$ divides the summation and every coefficient except $g_r h_t$ is divisible by $p$, we know that $p$ must also divide $g_r h_t$. -->

    <!-- \item Continuing from (b), we know that $p$ dividing $g_r h_t$ is a contradiction, since $p \nmid g_r$ nor $p \nmid h_t$. Thus, $p$ divides all of the coefficients of $G(x)$ or all of the coefficients of $H(x)$. $\blacksquare$ -->
<!-- \end{enumerate} -->

<!-- \section*{Problem 33} -->
<!-- Suppose that $f(x) \in \mathbb{Z}[x]$ is reducible over $\mathbb{Q}$, so $f(x) = b(x) c(x)$ where $b(x), c(x) \in \mathbb{Q}[x]$. Consider $k \in \mathbb{Z}$ such that $k$ is the least common multiple of the denominators of the coefficients in $b(x)$. Consider $l \in \mathbb{Z}$ such that $l$ is the least common multiple of the denominators of the coefficients in $c(x)$. Then, we know that $kb(x)$ and $lc(x)$ have integer coefficients, and we have: -->
<!-- $$klf(x) = (kb(x))(lc(x))$$ -->
<!-- Let $B(x), C(x) \in \mathbb{Z}[x]$ such that $B(x) = kb(x)$ and $C(x) = lc(x)$. Then, we get: -->
<!-- $$klf(x) = B(x) C(x)$$ -->
<!-- Since $k, l$ are integers, we know that $kl = p_1^{\alpha_1}p_2^{\alpha_2} \dots p_n^{\alpha_n}$, where $n \in \mathbb{N}$, $\alpha_1, \alpha_2, \dots, \alpha_n \in \mathbb{N}$, and $p_1, p_2, \dots, p_n$ are distinct primes. Hence, by \textbf{Lemma 2.27}, since $p_1$ divides all the coefficients of $f(x)$, $p_1$ divides all the coefficients of $B(x)$ or of $C(x)$. WLOG, we can apply the same reasoning for $p_2, \dots, p_n$ and for any power of these primes. Thus, we get: -->
<!-- $$f(x) = B'(x) C'(x)$$ -->
<!-- where $B'(x), C'(x) \in \mathbb{Z}[x]$. $\blacksquare$ -->

<!-- \section*{Problem 34} -->
<!-- Based on \textbf{Theorem 2.28}, consider $p = 3$. Since 3 divides $\{-12, -15, 6\}$, 3 does not divide 2, and 9 does not divide 12, we know that $f(x)$ is irreducible over $\mathbb{Z}$, hence over $\mathbb{Q}$. $\blacksquare$ -->

<!-- \section*{Problem 35} -->
<!-- \begin{enumerate}[label=(\alph*)] -->
    <!-- \item First note that since $f(x) = B(x) C(x)$, we know that $a_0 = b_0 c_0$. Then, note that we have three cases: -->
    <!-- \begin{itemize} -->
        <!-- \item $p$ does not divide neither $b_0$ nor $c_0$: \\ -->
        <!-- Then, we have $p \nmid a_0$ which is a contradiction. \xmark -->
        <!-- \item $p$ divides either $b_0$ or $c_0$ but not both: \\ -->
        <!-- WLOG let $p \mid b_0$ and so $p \nmid c_0$. Then, we know that $p \mid a_0$ and $p^2 \nmid a_0$. This aligns with the Theorem. \cmark -->
        <!-- \item $p$ divides both $b_0$ and $c_0$: \\ -->
        <!-- Then, we have $p^2 \mid a_0$ which is a contradiction. \xmark -->
    <!-- \end{itemize} -->

    <!-- \item Note that since $f(x) = B(x) C(x)$, we know that $a_n = b_u c_v$. Then, if $p \mid c_v$, then $p \mid a_n$ which is a contradiction. Hence, $p \nmid c_v$. -->

    <!-- \item The expression is: -->
    <!-- $$a_k = b_0 c_k + b_1 c_{k-1} + \dots + b_k c_0 = \sum_{i=0}^{k} b_i c_{k-i}$$ -->

    <!-- \item Since $k < n$, by the Theorem, we know that $p \mid a_k$. If we look at the expression of $a_k$ in (c), we see that every term in the summation except $b_0 c_k$ is divisible by $p$, because $p \mid c_j$ for all $0 \leq j < k$. Hence, $b_0 c_k$ must be also divisible by $p$. This is a contradiction. $\blacksquare$ -->
<!-- \end{enumerate} -->

<!-- \section*{Problem 36} -->
<!-- \begin{enumerate}[label=(\alph*)] -->
    <!-- \item is fine, by induction or multiply by $x-1$ -->

    <!-- \item $$\Phi_p(x+1) = \frac{(x+1)^p-1}{x}$$ -->
    <!-- By binomial theorem, $(x+1)^p = \sum_{k=0}^{n} {p \choose k} x^k$, and so the expressions for $(x+1)^p$ follows. -->

    <!-- \item By ${p \choose n} = \frac{p!}{n!(p-n)!}$, $p \mid {p \choose n}$ so long as $n \neq 0$ and $n \neq p$. And, ${p \choose p-1} = p$, so $p^2 \nmid {p \choose p-1}$. Lastly, $p \nmid 1$, so $\Phi_p(x+1)$ satisfies Eisenstein's Irreducibility Criterion and so is irreducible. -->

    <!-- \item Assume for contradiction $\Phi_p(x)$ is reducible. Then, $\Phi_p(x) = g(x)h(x)$, so $\Phi_p(x+1) = g(x+1)h(x+1)$, giving that $\Phi_p(x+1)$ is reducible, a contradiction. -->
<!-- \end{enumerate} -->

<!-- \vspace{5mm} -->

<!-- \noindent \textbf{Tiny little part of vector space (Chapter 3)} -->

<!-- \section*{Problem 3} -->
<!-- $E$ is the vector space ($V$), and $F$ is the field ($F$). -->
<!-- \begin{itemize} -->
    <!-- \item Define the addition operation in the vector space as the addition operation of $E$ as a field. Then, by $E$ a ring, $(E, +)$ forms an abelian group. -->

    <!-- \item Define the scalar multiplication operation for the vector space by the multiplication between elements of $E$.  -->

    <!-- \item Then, properties (1) and (3) follows by the distributive property of rings. -->

    <!-- \item Property (2) follows from multiplication in a ring associative. -->

    <!-- \item Property (4) follows by taking the identity element of the vector space to be the identity element of the field.  -->
<!-- \end{itemize} -->



<!-- \end{document} -->

